veric/rmaps.v
@@ -10,38 +10,7 @@ Parameter some_address:address.
 (* Validity of traces.  The "valid" predicate ensures that related addresses don't get
     split apart from each other.  *)
 Parameter kind: Type.
-Parameter valid : (address -> option (rshare * kind)) -> Prop.
-Parameter valid_empty: valid (fun _ => None).
-Parameter valid_join: forall f g h : address -> option (rshare * kind),
-   @join _ (Join_fun address (option (rshare * kind))
-                   (Join_lower (Join_prod rshare Join_rshare kind (Join_equiv kind))))
-      f g h  ->
- valid f -> valid g -> valid h.
 End ADR_VAL.
-
-Module Type ADR_VAL0.
-Parameter address : Type.
-Parameter some_address:address.
-Parameter kind: Type.
-End ADR_VAL0.
-
-Module SimpleAdrVal (AV0: ADR_VAL0) <:
-   ADR_VAL with Definition address := AV0.address
-                   with Definition kind := AV0.kind.
-  Import AV0.
-  Definition address := address.
-  Definition some_address := some_address.
-  Definition kind := kind.
-  Definition valid (_: address -> option (rshare * kind)) := True.
-  Lemma valid_empty: valid (fun _ => None).
-  Proof. unfold valid; auto. Qed.
-  Lemma valid_join: forall f g h : address -> option (rshare * kind),
-   @join _ (Join_fun address (option (rshare * kind))
-                   (Join_lower (Join_prod rshare Join_rshare kind (Join_equiv kind))))
-      f g h  ->
-    valid f -> valid g -> valid h.
-  Proof.  intros; unfold valid; auto. Qed.
-End SimpleAdrVal.
 
 Inductive TypeTree: Type :=
   | ConstType: Type -> TypeTree
@@ -187,20 +156,11 @@ Module Type STRAT_MODEL.
   Defined.
   Axiom paf_ghost : @pafunctor f_ghost ghost_join.
 
-  Definition valid' A (w: (address -> res A) * ghost A) : Prop :=
-    AV.valid (fun l => res_option A (fst w l)).
-
-  Axiom valid'_res_map : forall A B f g m,
-    valid' A m -> valid' B (fmap f_res f g oo fst m, fmap f_ghost f g (snd m)).
-
   Definition f_pre_rmap : functor :=
-    fsubset (fpair (ffunc (fconst address) f_res) f_ghost) _ valid'_res_map.
-
-  Axiom valid'_res_map2 : forall A B f g m,
-    valid' B (fmap f_res f g oo fst m, fmap f_ghost f g (snd m)) -> valid' A m.
+    fpair (ffunc (fconst address) f_res) f_ghost.
 
   Instance Join_pre_rmap (A: Type) : Join (f_pre_rmap A) :=
-            Join_prop _ (Join_prod _ (Join_fun address (res A) (res_join A)) _ (ghost_join A)) (valid' A).
+            Join_prod _ (Join_fun address (res A) (res_join A)) _ (ghost_join A).
 
   Declare Instance Perm_pre_rmap: forall (A: Type), Perm_alg (f_pre_rmap A).
   Declare Instance Sep_pre_rmap: forall (A: Type), Sep_alg (f_pre_rmap A).
@@ -208,8 +168,26 @@ Module Type STRAT_MODEL.
 
   Existing Instance ghost_join.
   Instance Join_res A : Join (f_res A) := res_join A.
-  Axiom pre_rmap_core: forall A (m : f_pre_rmap A),
-    exists P, core m = exist (valid' A) (core (proj1_sig m)) P.
+
+Axiom pre_rmap_core:
+forall (A : Type) (m : f_pre_rmap A),
+  @core (f_pre_rmap A) (Join_pre_rmap A) (Sep_pre_rmap A) m =
+ (@core ((fpair (ffunc (fconst address) f_res) f_ghost) A)
+           (Join_prod ((ffunc (fconst address) f_res) A)
+              (Join_pi ((fconst address) A)
+                 (fun _ : (fconst address) A => f_res A)
+                 (fun _ : (fconst address) A => Join_res A))
+              (f_ghost A) (ghost_join A))
+           (@Sep_prod ((ffunc (fconst address) f_res) A)
+              (Join_pi ((fconst address) A)
+                 (fun _ : (fconst address) A => f_res A)
+                 (fun _ : (fconst address) A => Join_res A))
+              (f_ghost A) (ghost_join A)
+              (Sep_pi ((fconst address) A)
+                 (fun _ : (fconst address) A => f_res A)
+                 (fun _ : (fconst address) A => Join_res A)
+                 (fun _ : (fconst address) A => sa_rj A)) 
+              (sa_gj A)) m).
 
 End STRAT_MODEL.
 
@@ -558,93 +536,46 @@ Module StratModel (AV' : ADR_VAL) : STRAT_MODEL with Module AV:=AV'.
         destruct o, o0; auto; contradiction.
   Qed.
 
-  Definition valid' A (w: (address -> res A) * ghost A) : Prop :=
-    AV.valid (fun l => res_option A (fst w l)).
-
-  Lemma same_valid : forall f1 f2, (forall x, f1 x = f2 x) -> AV.valid f1 -> AV.valid f2.
-  Proof.
-    intros; replace f2 with f1; trivial.
-    apply extensionality; auto.
-  Qed.
-
-  Lemma valid'_res_map : forall A B f g m,
-    valid' A m -> valid' B (fmap f_res f g oo fst m, fmap f_ghost f g (snd m)).
-  Proof.
-    unfold valid'; intros A B f g m.
-    apply same_valid; intro l.
-    unfold compose; simpl.
-    destruct (fst m l); simpl; auto.
-  Qed.
-
-  Lemma valid'_res_map2 : forall A B f g m,
-    valid' B (fmap f_res f g oo fst m, fmap f_ghost f g (snd m)) -> valid' A m.
-  Proof.
-    unfold valid'; intros A B f g m.
-    apply same_valid; intro l.
-    unfold compose; simpl.
-    destruct (fst m l) eqn: Hl; setoid_rewrite Hl; auto.
-  Qed.
-
-  Definition pre_rmap (A:Type) := { m:(address -> res A) * ghost A | valid' A m }.
+  Definition pre_rmap (A:Type) := ((address -> res A) * ghost A)%type.
   Definition f_pre_rmap : functor :=
-    fsubset (fpair (ffunc (fconst address) f_res) f_ghost) _ valid'_res_map.
+    fpair (ffunc (fconst address) f_res) f_ghost.
 
   Notation Join_obj A := (Join_prod _ (Join_fun address (res A) (res_join A)) _ (ghost_join A)).
 
   Instance Join_pre_rmap (A: Type) : Join (pre_rmap A) :=
-    Join_prop _ (Join_obj A) (valid' A).
+    Join_obj A.
 
   Definition paf_pre_rmap : @pafunctor f_pre_rmap Join_pre_rmap :=
-    paf_subset (paf_pair (paf_fun address paf_res) paf_ghost) valid' valid'_res_map valid'_res_map2.
-
-  Lemma pre_rmap_sa_valid_core (A: Type):
-        forall x,
-       valid' A x ->
-       valid' A  (@core ((address -> res A) * ghost A) (Join_obj A)
-         (Sep_prod (Sep_fun address (res A) (res_join A) (sa_rj A)) (sa_gj A)) x).
-  Proof.
-    intros. red. red.
-    replace (fun l => res_option A (fst (core x) l)) with (fun l : address => @None (rshare * kind)).
-    apply AV.valid_empty.
-    extensionality a. simpl. icase (fst x a).
-  Qed.
-
-
-  Lemma pre_rmap_sa_valid_join : forall A (x y z : (address -> res A) * ghost A),
-    @join _ (Join_obj A) x y z ->
-    valid' A x -> valid' A y -> valid' A z.
-  Proof.
-     intros.
-     simpl in H.
-     unfold valid' in *.
-     apply AV.valid_join with (fun l => res_option A (fst x l)) (fun l => res_option A (fst y l)); auto.
-     intro l. inv H.
-     specialize ( H2 l). inv H2; try constructor; simpl.
-     - apply join_comm in H6.
-       rewrite (join_readable_part_eq rsh2 nsh1 rsh3 H6). constructor.
-     - rewrite (join_readable_part_eq rsh1 nsh2 rsh3 H6). constructor.
-     - constructor.
-       red. red. simpl.
-       clear - H6. destruct H6. split.
-       + rewrite Share.glb_assoc. rewrite <- (Share.glb_assoc sh1).
-         rewrite (Share.glb_commute sh1). rewrite Share.glb_assoc.
-         rewrite <- (Share.glb_assoc Share.Rsh).
-         rewrite H. rewrite Share.glb_bot. auto.
-       + rewrite <- Share.distrib1. rewrite H0. auto.
-       + constructor. reflexivity. reflexivity.
-  Qed.
+    paf_pair (paf_fun address paf_res) paf_ghost.
 
   Definition Perm_pre_rmap (A: Type): Perm_alg (pre_rmap A) :=
-    Perm_prop _ _ (Perm_prod (Perm_fun address _ _ _) (pa_gj A)) _ (pre_rmap_sa_valid_join _).
+    Perm_prod (Perm_fun address _ _ _) (pa_gj A).
 
-  Instance Sep_pre_rmap (A: Type): Sep_alg (pre_rmap A) :=
-    Sep_prop _ _ (Perm_prod (Perm_fun address _ _ _) (pa_gj A)) _ (pre_rmap_sa_valid_join _)  _ (pre_rmap_sa_valid_core _).
+  Definition Sep_pre_rmap (A: Type): Sep_alg (pre_rmap A) :=
+    Sep_prod (Sep_fun address _ _ _) (sa_gj A).
 
-  Lemma pre_rmap_core: forall A (m : f_pre_rmap A),
-    exists P, core m = exist (valid' A) (core (proj1_sig m)) P.
-  Proof.
-    simpl; eauto.
-  Qed.
+Lemma pre_rmap_core:
+forall (A : Type) (m : f_pre_rmap A),
+  @core (f_pre_rmap A) (Join_pre_rmap A) (Sep_pre_rmap A) m =
+ (@core ((fpair (ffunc (fconst address) f_res) f_ghost) A)
+           (Join_prod ((ffunc (fconst address) f_res) A)
+              (Join_pi ((fconst address) A)
+                 (fun _ : (fconst address) A => f_res A)
+                 (fun _ : (fconst address) A => Join_res A))
+              (f_ghost A) (ghost_join A))
+           (@Sep_prod ((ffunc (fconst address) f_res) A)
+              (Join_pi ((fconst address) A)
+                 (fun _ : (fconst address) A => f_res A)
+                 (fun _ : (fconst address) A => Join_res A))
+              (f_ghost A) (ghost_join A)
+              (Sep_pi ((fconst address) A)
+                 (fun _ : (fconst address) A => f_res A)
+                 (fun _ : (fconst address) A => Join_res A)
+                 (fun _ : (fconst address) A => sa_rj A)) 
+              (sa_gj A)) m).
+Proof.
+intros. reflexivity.
+Qed.
 
 End StratModel.
 
@@ -744,18 +675,11 @@ Module Type RMAPS.
   Axiom ghost_fmap_comp : forall f1 f2 g1 g2,
     ghost_fmap g1 g2 oo ghost_fmap f1 f2 = ghost_fmap (g1 oo f1) (f2 oo g2).
 
-  Definition valid (m: (address -> resource) * ghost) : Prop :=
-    AV.valid  (res_option oo fst m).
-
-  Axiom valid_res_map : forall f g m, valid m -> valid (resource_fmap f g oo fst m, ghost_fmap f g (snd m)).
-  Axiom rmapj_valid_join : forall (x y z : (address -> resource) * ghost),
-    join x y z -> valid x -> valid y -> valid z.
-  Axiom rmapj_valid_core: forall x: (address -> resource) * ghost, valid x -> valid (core x).
-
-  Definition rmap' := sig valid.
+  Definition rmap' := ((address -> resource) * ghost)%type.
 
   Definition rmap_fmap (f g: pred rmap -> pred rmap) (x:rmap') : rmap' :=
-    match x with exist m H => exist (fun m => valid m) (resource_fmap f g oo fst m, ghost_fmap f g (snd m)) (valid_res_map f g m H) end.
+    (resource_fmap f g oo fst x, ghost_fmap f g (snd x)).
+
   Axiom rmap_fmap_id : rmap_fmap (id _) (id _) = id rmap'.
   Axiom rmap_fmap_comp : forall f1 f2 g1 g2,
    rmap_fmap g1 g2 oo rmap_fmap f1 f2 = rmap_fmap (g1 oo f1) (f2 oo g2).
@@ -771,9 +695,9 @@ Module Type RMAPS.
     | (S n,x) => Some (squash (n,x))
     end.
 
-  Definition resource_at (phi:rmap) : address -> resource := fst (proj1_sig (snd (unsquash phi))).
+  Definition resource_at (phi:rmap) : address -> resource := fst (snd (unsquash phi)).
   Infix "@" := resource_at (at level 50, no associativity).
-  Definition ghost_of (phi:rmap) : ghost := snd (proj1_sig (snd (unsquash phi))).
+  Definition ghost_of (phi:rmap) : ghost := snd (snd (unsquash phi)).
 
   Instance Join_nat_rmap': Join (nat * rmap') := Join_prod _ (Join_equiv nat) _ _.
 
@@ -904,9 +828,6 @@ Module Rmaps (AV':ADR_VAL): RMAPS with Module AV:=AV'.
     rewrite IHx; destruct a as [[]|]; auto; simpl.
     destruct p; auto.
   Qed.
-
-  Definition valid (m: (address -> resource) * ghost) : Prop :=
-    AV.valid  (res_option oo fst m).
 
   Inductive res_join : resource -> resource -> resource -> Prop :=
    | res_join_NO1 : forall sh1 nsh1 sh2 nsh2 sh3 nsh3
@@ -1095,49 +1016,7 @@ Module Rmaps (AV':ADR_VAL): RMAPS with Module AV:=AV'.
     auto.
   Qed.
 
-  Lemma same_valid : forall f1 f2, (forall x, f1 x = f2 x) -> AV.valid f1 -> AV.valid f2.
-  Proof.
-    intros; replace f2 with f1; trivial.
-    apply extensionality; auto.
-  Qed.
-
-  Lemma rmapj_valid_core: forall x : (address -> resource) * ghost, valid x -> valid (core x).
-  Proof.
-     unfold valid, compose; intros. red. red. 
-     replace (fun x0 => res_option (fst (core x) x0)) with (fun _ : address => @None (rshare * kind)).
-
-     apply AV.valid_empty.
-     extensionality a. simpl. icase (fst x a).
-  Qed.
-
-  Lemma rmapj_valid_join : forall (x y z : (address -> resource) * ghost),
-    join x y z ->
-    valid x -> valid y -> valid z.
-  Proof.
-     intros.
-     simpl in H.
-     unfold valid, compose in *.
-     apply AV.valid_join with (fun l => res_option (fst x l)) (fun l => res_option (fst y l)); auto.
-     intro l. inv H. specialize (H2 l). inv H2; eauto.
-     - constructor.
-     - simpl.
-       rewrite (join_readable_part_eq rsh1 nsh2 rsh3 RJ). constructor.
-     - apply join_comm in RJ.
-       simpl.
-       rewrite (join_readable_part_eq rsh2 nsh1 rsh3 RJ). constructor.
-     - constructor. constructor.
-       + simpl. red. red. simpl.
-         clear - RJ. destruct RJ. split.
-         * rewrite Share.glb_assoc. rewrite <- (Share.glb_assoc sh1).
-           rewrite (Share.glb_commute sh1). rewrite Share.glb_assoc.
-           rewrite <- (Share.glb_assoc Share.Rsh).
-           rewrite H. rewrite Share.glb_bot. auto.
-         * rewrite <- Share.distrib1. rewrite H0. auto.
-       + constructor; reflexivity.
-    - constructor.
-  Qed.
-
-  Definition rmap' := sig valid.
+  Definition rmap' := ((address->resource) * ghost)%type.
   Definition preds_fmap (f g:(pred rmap)->(pred rmap)) (x:preds) : preds :=
     match x with SomeP A ls => SomeP A (fmap (fpi _) f g ls) end.
 
@@ -1169,16 +1048,6 @@ Module Rmaps (AV':ADR_VAL): RMAPS with Module AV:=AV'.
 
   Definition ghost_fmap (f g:pred rmap -> pred rmap)(x:ghost) : ghost :=
     map (option_map (fun '(a, b) => (a, preds_fmap f g b))) x.
-
-  Lemma valid_res_map : forall f g m, valid m -> valid (resource_fmap f g oo fst m, ghost_fmap f g (snd m)).
-  Proof.
-    unfold valid, compose; intros; simpl.
-    replace (fun l : address => res_option (resource_fmap f g (fst m l)))
-       with (fun l : address => res_option (fst m l)); auto.
-    extensionality l.
-    unfold res_option, resource_fmap.
-    case (fst m l); auto.
-  Qed.
 
   Lemma resource_fmap_id :
     resource_fmap (id (pred rmap)) (id (pred rmap)) = id resource.
@@ -1216,17 +1085,16 @@ Module Rmaps (AV':ADR_VAL): RMAPS with Module AV:=AV'.
   Qed.
 
   Definition rmap_fmap (f g:(pred rmap)->(pred rmap)) (x:rmap') : rmap' :=
-    match x with exist m H => exist (fun m => valid m) _ (valid_res_map f g m H) end.
+              (resource_fmap f g oo fst x, ghost_fmap f g (snd x)).
 
   Lemma rmap_fmap_id : rmap_fmap (id (pred rmap)) (id (pred rmap)) = id rmap'.
   Proof.
     intros; apply extensionality; intro x.
     unfold rmap_fmap; destruct x.
-    unfold id at 7.
-    generalize (valid_res_map (id _) (id _) x v).
+    simpl.
     rewrite resource_fmap_id, ghost_fmap_id.
-    rewrite (id_unit2 _ (resource) (fst x)).
-    intro v0. destruct x; simpl. f_equal; auto. apply proof_irr.
+    rewrite (id_unit2 _ (resource) r).
+    f_equal; auto.
   Qed.
 
   Lemma rmap_fmap_comp : forall f1 f2 g1 g2,
@@ -1236,51 +1104,27 @@ Module Rmaps (AV':ADR_VAL): RMAPS with Module AV:=AV'.
     unfold rmap_fmap.
     apply extensionality; intro x.
     unfold compose at 1.
-    destruct x.
-    generalize (valid_res_map g1 g2 (resource_fmap f1 f2 oo fst x, ghost_fmap f1 f2 (snd x)) (valid_res_map f1 f2 x v)).
-    generalize (valid_res_map (g1 oo f1) (f2 oo g2) x v).
-    clear.
-    assert (resource_fmap g1 g2 oo resource_fmap f1 f2 oo fst x = resource_fmap (g1 oo f1) (f2 oo g2) oo fst x).
-    { rewrite <- compose_assoc.
-      rewrite resource_fmap_comp; auto. }
-    simpl; rewrite H.
+    destruct x as (r,g). simpl.
+    rewrite <- compose_assoc.
+    rewrite resource_fmap_comp; auto.
+    f_equal; auto.
     pose proof ghost_fmap_comp as HG.
     unfold compose in HG at 1; rewrite <- HG.
     intros.
     f_equal; proof_irr; auto.
   Qed.
 
-  Definition rmap'2pre_rmap (r: rmap') : f_pre_rmap (pred rmap).
-    destruct r as [f ?].
-    unfold f_pre_rmap.
-    assert (valid' _ (fun x: address => resource2res (fst f x), ghost2g (snd f))).
-    unfold valid'. unfold valid, compose in v.
-    eapply same_valid; try apply v.
-    intros. simpl.
-    destruct (fst f x); simpl; auto; destruct p; simpl; auto.
-    eexists. exact H.
-  Defined.
+  Definition rmap'2pre_rmap (f: rmap') : f_pre_rmap (pred rmap) :=
+      (fun x : address => resource2res (fst f x), ghost2g (snd f)).
 
-  Definition pre_rmap2rmap' (r: f_pre_rmap (pred rmap)) : rmap'.
-    destruct r as [f ?].
-    unfold rmap', valid' in *.
-    assert (valid (fun l: address => res2resource (fst f l), g2ghost (snd f))).
-    unfold valid, compose.
-    simpl.
-    assert ((fun l : address => res_option (res2resource (fst f l))) = (fun l : address => SM.res_option (pred rmap) (fst f l))).
-    { extensionality l. rewrite res_option_rewrite.
-      unfold compose; simpl. rewrite res2resource2res. auto. }
-    setoid_rewrite H; auto.
-    eauto.
-  Defined.
+  Definition pre_rmap2rmap' (f: f_pre_rmap (pred rmap)) : rmap' :=
+      (fun l : address => res2resource (fst f l), g2ghost (snd f)).
 
   Lemma rmap'2pre_rmap2rmap' :
     forall x, rmap'2pre_rmap (pre_rmap2rmap' x) = x.
   Proof.
-    intro. destruct x as [f V]. unfold rmap'2pre_rmap, pre_rmap2rmap'. simpl.
-    match goal with |- exist _ _ ?p = _ => generalize p; intro p1 end.
-    apply exist_ext.
-    destruct f; simpl; f_equal.
+    intro. unfold rmap'2pre_rmap, pre_rmap2rmap'. simpl.
+    destruct x; simpl; f_equal.
     extensionality x; rewrite res2resource2res; auto.
     rewrite g2ghost2g; auto.
   Qed.
@@ -1289,30 +1133,12 @@ Module Rmaps (AV':ADR_VAL): RMAPS with Module AV:=AV'.
     forall x,  pre_rmap2rmap' (rmap'2pre_rmap x) = x.
   Proof.
     intro.
-    destruct x as [f V].
     unfold rmap'2pre_rmap, pre_rmap2rmap'. simpl.
-    match goal with |- exist _ _ ?p = _ => generalize p; intro p1 end.
-    apply exist_ext.
-    destruct f; simpl; f_equal.
+    destruct x; simpl; f_equal.
     extensionality x; rewrite resource2res2resource; auto.
     rewrite ghost2g2ghost; auto.
   Qed.
-(*
-  Program Definition p2p (p:(pred rmap)) : K.predicate :=
-    fun phi_e => p phi_e.
-  Next Obligation.
-    unfold age, age1 in H. simpl in H. simpl in *.
-    eapply pred_hereditary; eauto.
- Qed.
 
-  Program Definition p2p' (p:K.predicate) : (pred rmap) :=
-    fun (v:rmap) => p v.
-  Next Obligation.
-  unfold age in H; simpl in H.
-  unfold rmap in *.
-  eapply pred_hereditary; eauto.
- Qed.
-*)
   Definition squash (n_rm:nat * rmap') : rmap :=
     match n_rm with (n,rm) => K.squash (n, rmap'2pre_rmap rm) end.
 
@@ -1320,9 +1146,9 @@ Module Rmaps (AV':ADR_VAL): RMAPS with Module AV:=AV'.
     match K.unsquash phi with (n,rm) => (n, pre_rmap2rmap' rm) end.
 
   Definition rmap_level (phi:rmap) : nat := fst (unsquash phi).
-  Definition resource_at (phi:rmap) : address -> resource := fst (proj1_sig (snd (unsquash phi))).
+  Definition resource_at (phi:rmap) : address -> resource := fst (snd (unsquash phi)).
   Infix "@" := resource_at (at level 50, no associativity).
-  Definition ghost_of (phi:rmap) : ghost := snd (proj1_sig (snd (unsquash phi))).
+  Definition ghost_of (phi:rmap) : ghost := snd (snd (unsquash phi)).
 
   Lemma pred_ext': forall {A} `{agA: ageable A} P Q,
                 (forall x, app_pred P x <-> app_pred Q x) -> P = Q.
@@ -1377,9 +1203,7 @@ Module Rmaps (AV':ADR_VAL): RMAPS with Module AV:=AV'.
     end.
     2: repeat rewrite <- fmap_comp.
     2: unfold compose; auto.
-    destruct rm; simpl.
-    apply exist_ext.
-    destruct x; simpl; f_equal.
+    destruct rm; simpl. unfold pre_rmap2rmap', rmap_fmap. simpl; f_equal.
     extensionality l.
     unfold compose.
     destruct (r l); simpl; auto.
@@ -1390,7 +1214,7 @@ Module Rmaps (AV':ADR_VAL): RMAPS with Module AV:=AV'.
     destruct p; simpl.
     rewrite approx_K_approx; auto.
     (* ghost *)
-    clear v; induction g; auto; simpl.
+    induction g; auto; simpl.
     setoid_rewrite IHg; destruct a as [[]|]; auto; simpl.
     repeat f_equal.
     rewrite approx_K_approx; destruct p; auto.
@@ -1442,9 +1266,6 @@ Qed.
     inversion H0.
     constructor.
     intro l; specialize ( H1 l).
-    destruct f as [f ?].
-    destruct f0 as [f0 ?].
-    destruct f1 as [f1 ?].
     simpl in *.
     unfold compose.
     destruct f, f0, f1; simpl in *.
@@ -1456,17 +1277,13 @@ Qed.
     destruct p; simpl in *.
     constructor; auto.
 
-    destruct f, f0, f1; simpl in *.
-    destruct x, x0, x1; simpl in *.
+    destruct f, f0, f1; simpl in *. 
     clear - H2; induction H2; constructor; auto.
     inv H; constructor; auto.
     destruct a0, a4, a5; inv H0; simpl in *.
     inv H; inv H1; constructor; constructor; auto.
 
     destruct H; simpl in *; split; simpl; auto.
-    destruct f as [f ?].
-    destruct f0 as [f0 ?].
-    destruct f1 as [f1 ?].
     inversion H0.
     hnf in H1. simpl proj1_sig in H1.
     constructor; auto.
@@ -1516,10 +1333,9 @@ Qed.
     intro; rewrite KSa.core_unsquash.
     unfold ghost_of, KSa.K.unsquash, KSa.K.squash, unsquash, squash.
     destruct (K.unsquash phi); simpl.
-    rewrite K.unsquash_squash.
-    destruct (pre_rmap_core _ _f).
-    setoid_rewrite H; auto.
-  Qed.
+    rewrite K.unsquash_squash; simpl.
+    setoid_rewrite (pre_rmap_core _ _f). auto.
+Qed.
 
   Definition rmap_age1 (k:rmap) : option rmap :=
     match unsquash k with
